update correctness theorem

examples/pseudo_bool/array/compilation/proofs/cnfProofScript.sml
@@ -11,29 +11,29 @@ open preamble
 
 val _ = new_theory"cnfProof";
 
-val main_io_events_def = new_specification("main_io_events_def",["main_io_events"],
+val cake_pb_cnf_io_events_def = new_specification("cake_pb_cnf_io_events_def",["cake_pb_cnf_io_events"],
   main_semantics |> Q.GENL[`cl`,`fs`]
   |> SIMP_RULE bool_ss [SKOLEM_THM,Once(GSYM RIGHT_EXISTS_IMP_THM)]);
 
-val (main_sem,main_output) = main_io_events_def |> SPEC_ALL |> UNDISCH |> SIMP_RULE std_ss [GSYM PULL_EXISTS]|> CONJ_PAIR
-val (main_not_fail,main_sem_sing) = MATCH_MP semantics_prog_Terminate_not_Fail main_sem |> CONJ_PAIR
+val (cake_pb_cnf_sem,cake_pb_cnf_output) = cake_pb_cnf_io_events_def |> SPEC_ALL |> UNDISCH |> SIMP_RULE std_ss [GSYM PULL_EXISTS]|> CONJ_PAIR
+val (cake_pb_cnf_not_fail,cake_pb_cnf_sem_sing) = MATCH_MP semantics_prog_Terminate_not_Fail cake_pb_cnf_sem |> CONJ_PAIR
 
 val compile_correct_applied =
   MATCH_MP compile_correct cnf_compiled
   |> SIMP_RULE(srw_ss())[LET_THM,ml_progTheory.init_state_env_thm,GSYM AND_IMP_INTRO]
-  |> C MATCH_MP main_not_fail
+  |> C MATCH_MP cake_pb_cnf_not_fail
   |> C MATCH_MP x64_backend_config_ok
-  |> REWRITE_RULE[main_sem_sing,AND_IMP_INTRO]
+  |> REWRITE_RULE[cake_pb_cnf_sem_sing,AND_IMP_INTRO]
   |> REWRITE_RULE[Once (GSYM AND_IMP_INTRO)]
   |> C MATCH_MP (CONJ(UNDISCH x64_machine_config_ok)(UNDISCH x64_init_ok))
   |> DISCH(#1(dest_imp(concl x64_init_ok)))
   |> REWRITE_RULE[AND_IMP_INTRO]
 
-val main_compiled_thm =
-  CONJ compile_correct_applied main_output
+val cake_pb_cnf_compiled_thm =
+  CONJ compile_correct_applied cake_pb_cnf_output
   |> DISCH_ALL
   (* |> check_thm *)
-  |> curry save_thm "main_compiled_thm";
+  |> curry save_thm "cake_pb_cnf_compiled_thm";
 
 (* Prettifying the standard parts of all the theorems *)
 val installed_x64_def = Define `
@@ -50,23 +50,23 @@ val installed_x64_def = Define `
         (heap_regs x64_backend_config.stack_conf.reg_names) mc ms
     `;
 
-val main_code_def = Define `
-  main_code = (code, data, config)
+val cake_pb_cnf_code_def = Define `
+  cake_pb_cnf_code = (code, data, config)
   `;
 
 (* A standard run of cake_lpr satisfying all the default assumptions *)
-val cake_lpr_run_def = Define`
-  cake_lpr_run cl fs mc ms ⇔
+val cake_pb_cnf_run_def = Define`
+  cake_pb_cnf_run cl fs mc ms ⇔
   wfcl cl ∧ wfFS fs ∧ STD_streams fs ∧ hasFreeFD fs ∧
-  installed_x64 main_code mc ms`
+  installed_x64 cake_pb_cnf_code mc ms`
 
 Theorem machine_code_sound:
-  cake_lpr_run cl fs mc ms ⇒
+  cake_pb_cnf_run cl fs mc ms ⇒
   machine_sem mc (basis_ffi cl fs) ms ⊆
     extend_with_resource_limit
-      {Terminate Success (main_io_events cl fs)} ∧
+      {Terminate Success (cake_pb_cnf_io_events cl fs)} ∧
   ∃out err.
-    extract_fs fs (main_io_events cl fs) =
+    extract_fs fs (cake_pb_cnf_io_events cl fs) =
       SOME (add_stdout (add_stderr fs err) out) ∧
   if out = strlit "s VERIFIED UNSAT\n" then
     LENGTH cl = 3 ∧
@@ -77,8 +77,8 @@ Theorem machine_code_sound:
   else out = strlit ""
 Proof
   strip_tac>>
-  fs[installed_x64_def,main_code_def,cake_lpr_run_def]>>
-  drule main_compiled_thm>>
+  fs[installed_x64_def,cake_pb_cnf_code_def,cake_pb_cnf_run_def]>>
+  drule cake_pb_cnf_compiled_thm>>
   simp[AND_IMP_INTRO]>>
   disch_then drule>>
   disch_then (qspecl_then [`ms`,`mc`,`data_sp`,`cbspace`] mp_tac)>>
